\documentclass[12pt]{article}
\usepackage{pmmeta}
\pmcanonicalname{BoundOnMatrixDifferentialEquation}
\pmcreated{2013-03-22 18:59:00}
\pmmodified{2013-03-22 18:59:00}
\pmowner{rspuzio}{6075}
\pmmodifier{rspuzio}{6075}
\pmtitle{bound on matrix differential equation}
\pmrecord{4}{41848}
\pmprivacy{1}
\pmauthor{rspuzio}{6075}
\pmtype{Theorem}
\pmcomment{trigger rebuild}
\pmclassification{msc}{34A30}

\endmetadata

% this is the default PlanetMath preamble.  as your knowledge
% of TeX increases, you will probably want to edit this, but
% it should be fine as is for beginners.

% almost certainly you want these
\usepackage{amssymb}
\usepackage{amsmath}
\usepackage{amsfonts}

% used for TeXing text within eps files
%\usepackage{psfrag}
% need this for including graphics (\includegraphics)
%\usepackage{graphicx}
% for neatly defining theorems and propositions
%\usepackage{amsthm}
% making logically defined graphics
%%%\usepackage{xypic}

% there are many more packages, add them here as you need them

% define commands here

\begin{document}
Suppose that $A$ and $Z$ are two square matrices dependent
on a parameter which satisfy the differential equation
\[
 Z'(t) = A(t) Z(t)
\]
withh initial condition $Z(0) = I$.
Letting $\| \cdot \|$ denote the matrix operator norm, we
will show that, if $\| A(t) \| \le C$ for some constant
$C$ when $0 \le t \le R$, then
\[
 \| Z(t) - I \| \le C \left( e^{Ct} - 1 \right)
\]
when $0 \le t \le R$.

We begin by applying the product inequality for the norm,
then employing the triangle inequality (both in the sum and
integral forms) after expressing
$Z$ as the integral of its derivative:
\begin{align*}
 \| Z'(t) \| &\le \| A(t) \| \| Z(t) \| \\
  & \le C \| Z(t) \| \\
  & = C \left\| I + \int_0^t ds \, Z'(s) \right\| \\
  &\le C \| I \| + C \int_0^t ds \, \| Z' (s) \| \\
  &\le C + C \int_0^t ds \, \| Z' (s) \|
\end{align*}

For convenience, let us define $f(t) = \int_0^t ds \, \| Z' (s) \|$.
Then we have $f'(t) \le C + C f(t)$ according to the 
foregoing derivation.  By the product rule,
\[
 {d \over dt} \left( e^{-Ct} f(t) \right) =
  e^{-Ct} (f'(t) - C f(t)) .
\]
Since $f'(t) - C f(t) \le C$, we have
\[
 {d \over dt} \left( e^{-Ct} f(t) \right) \le
  C e^{-Ct} .
\]
Taking the integral from $0$ to $t$ of both sides and 
noting that $f(0) = 0$, we have
\[
 e^{-Ct} f(t) \le C \left( 1 - e^{-Ct} \right) .
\]
Multiplying both sides by $e^{Ct}$ and recalling the
definition of $f$, we conclude
\[
 \int_0^t ds \, \| Z'(s) \| 
   \le C \left( e^{Ct} - 1 \right) .
\]

Finally, by the triangle inequality,
\[
 \| Z(t) - I \| 
   = \left\| \int_0^t ds \, Z(s) \right\|
   \le \int_0^t ds \, \| Z(s) \| .
\]
Combining this with the inequality derived in the
last paragraph produces the answer:
\[
 \| Z(t) - I \| \le C \left( e^{Ct} - 1 \right) .
\]
%%%%%
%%%%%
\end{document}
